examples/HolOmega/interim/g_adjointScript.sml
@@ -1,23 +1,20 @@
 (* $Id$ *)
+(* Modified to show the improve rewriting and resolution tactics,
+   and to provide type annotations for variables with universal types, by PVH *)
 structure g_adjointScript =
 struct
 
 open HolKernel Parse boolLib bossLib
 
-open categoryTheory KmonadTheory auxLib ; infix RS RSN ;
+open categoryTheory KmonadTheory auxLib boolSimps ;
+infix RS RSN ;
 val UNCURRY_DEF = pairTheory.UNCURRY_DEF ;
 val o_THM = combinTheory.o_THM ;
 val o_DEF = combinTheory.o_DEF ;
 val I_THM = combinTheory.I_THM ;
 
-(*
-load "auxLib" ;
-load "g_adjointTheory" ; open g_adjointTheory ;
-fun sge tm = set_goal ([], tm) ;
-fun eev tacs = e (EVERY tacs) ;
-fun eall [] = () 
-  | eall (t :: ts) = (e t ; eall ts) ;
-*)
+val combin_ss  = bool_ss ++ combinSimps.COMBIN_ss
+val satisfy_ss = bool_ss ++ SatisfySimps.SATISFY_ss
 
 val _ = set_trace "Unicode" 1;
 val _ = set_trace "kinds" 0;
@@ -25,9 +22,8 @@ val _ = set_trace "kinds" 0;
 val _ = new_theory "g_adjoint";
 
 (* 
-show_types := false ;
-show_types := true ;
-handle e => Raise e ;
+load "g_adjointTheory" ; open g_adjointTheory ; 
+load "auxLib" ; open auxLib ;
 *)
 
 val _ = type_abbrev ("g_sharp",
@@ -81,23 +77,23 @@ val g_adjf5_def = new_definition("g_adjf5_def",
 (* note, [:'b,'a:] required in g_adjf2_thm,
   [:'a,'b:] not required in g_adjf1_thm *)
 val g_adjf1_thm = store_thm ("g_adjf1_thm",
-  ``g_adjf1 [:'C,'D:] (idC,compC) G eta sharp =
+  ``g_adjf1 [:'C,'D, 'F, 'G:] (idC,compC) G eta sharp =
     (!: 'a 'b. (! (f : ('a, 'b 'G) 'C) g. 
       (compC (G g) eta = f) = (sharp [:'a,'b:] f = g)))``,
   SRW_TAC [] [g_adjf1_def]) ;
-				      
+
 val g_adjf2_thm = store_thm ("g_adjf2_thm",
-  ``g_adjf2 [:'D,'C:] (idD,compD) F' eps flatt =
+  ``g_adjf2 [:'D,'C, 'G,'F:] (idD,compD) F' eps flatt =
     (!: 'b 'a. (! g (f : ('a, 'b 'G) 'C). 
       (compD eps (F' f) = g) = (flatt [:'b,'a:] g = f)))``, 
   SRW_TAC [] [g_adjf2_def]) ;
-				      
+
 val g_adjf3_thm = store_thm ("g_adjf3_thm",
-  ``g_adjf3 [:'C,'D:] (idC,compC) (idD,compD) F' G eta eps =
+  ``g_adjf3 [:'C,'D, 'F,'G:] (idC,compC) (idD,compD) F' G eta eps =
     (!: 'a 'b. ! (f : ('a, 'b 'G) 'C) g. 
       (compC (G g) eta = f) = (compD eps (F' f) = g))``,
   SRW_TAC [] [g_adjf3_def]) ;
-				      
+
 val exp_convs = [ TY_BETA_CONV, BETA_CONV,
   HO_REWR_CONV pairTheory.FORALL_PROD, REWR_CONV UNCURRY_DEF,
   REWR_CONV TY_FUN_EQ_THM, REWR_CONV FUN_EQ_THM ] ; 
@@ -105,7 +101,7 @@ val exp_convs = [ TY_BETA_CONV, BETA_CONV,
 val mk_exp_thm = CONV_RULE (REDEPTH_CONV (FIRST_CONV exp_convs)) ;
 
 val g_adjf4_thm = save_thm ("g_adjf4_thm",
-  SPEC_ALL (TY_SPEC_ALL (mk_exp_thm g_adjf4_def))) ;
+  TY_TM_SPEC_ALL (mk_exp_thm g_adjf4_def)) ;
 
 val g_adjf5_thm = store_thm ("g_adjf5_thm",
   ``g_adjf5 [:'C, 'D, 'F, 'G:] (idC : 'C id, compC : 'C o_arrow)
@@ -122,44 +118,37 @@ val g_adjf3_dual = store_thm ("g_adjf3_dual",
   ``g_adjf3 [:'C, 'D, 'F, 'G:] (idC,compC) (idD,compD) F' G eta eps = 
     g_adjf3 [:'D C,'C C,'G,'F:] (idD, dual_comp compD) (idC, dual_comp compC) 
       (g_dual_functor G) (g_dual_functor F') eps eta``,
-  EVERY [ (REWRITE_TAC [dual_comp_def, g_dual_functor_def, g_adjf3_thm]),
-    TY_BETA_TAC, BETA_TAC, EQ_TAC, STRIP_TAC, (ASM_REWRITE_TAC []) ]) ;
-      
+  SIMP_TAC bool_ss [dual_comp_def, g_dual_functor_def, g_adjf3_thm]
+  THEN EQ_TAC THEN ASM_SIMP_TAC bool_ss []) ;
+
 val g_adjf12_dual = store_thm ("g_adjf12_dual",
   ``g_adjf2 [:'D,'C, 'G, 'F:] (idD,compD) F' eps flatt = 
     g_adjf1 [:'D C,'C C, 'G, 'F:] 
       (idD, dual_comp compD) (g_dual_functor F') eps flatt``,
-  EVERY [ 
-    (REWRITE_TAC [dual_comp_def, g_dual_functor_def, g_adjf1_thm, g_adjf2_thm]),
-    TY_BETA_TAC, BETA_TAC, REFL_TAC]) ;
+  SIMP_TAC bool_ss [dual_comp_def, g_dual_functor_def, g_adjf1_thm, g_adjf2_thm]) ;
 
 val g_adjf4_dual = store_thm ("g_adjf4_dual",
   ``g_adjf4 [:'C, 'D, 'F, 'G:] (idC,compC) (idD,compD) sharp flatt = 
     g_adjf4 [:'D C, 'C C, 'G, 'F:] 
       (idD, dual_comp compD) (idC, dual_comp compC) flatt sharp``,
-  EVERY [ (REWRITE_TAC [dual_comp_def, g_adjf4_thm]),
-    TY_BETA_TAC, BETA_TAC, EQ_TAC, STRIP_TAC, 
-    CONJ_TAC, REPEAT STRIP_TAC, 
-    TRY (FIRST_ASSUM MATCH_ACCEPT_TAC),
-    ASM_REWRITE_TAC [] ]) ;
-      
-(*
-show_types := true ;
-show_types := false ;
-handle e => Raise e ;
-set_goal ([], it) ;
-val (sgs, goal) = top_goal () ;
-*)
+  SIMP_TAC bool_ss [dual_comp_def, g_adjf4_thm]
+  THEN EQ_TAC THEN REPEAT STRIP_TAC
+  THEN TRY (FIRST_ASSUM MATCH_ACCEPT_TAC)
+  THEN ASM_REWRITE_TAC[]
+) ;
 
-val g_adjf1DGh' = prove (``g_adjf1 (idC, compC : 'C o_arrow) G eta sharp ==>
-    (compC (G (sharp f)) eta = f)``,
-  EVERY [ STRIP_TAC, (IMP_RES_TAC g_adjf1_thm), (ASM_REWRITE_TAC []) ]) ;
-
-val g_adjf1DGh = save_thm ("g_adjf1DGh",
-  DISCH_ALL (TY_GEN_ALL (GEN_ALL (UNDISCH g_adjf1DGh')))) ;
+val g_adjf1DGh = store_thm ("g_adjf1DGh", 
+  ``g_adjf1 [:'C,'D, 'F,'G:] (idC, compC : 'C o_arrow) G
+            (eta : ('C, I, 'F o 'G) g_nattransf) sharp ==>
+    (!:'a 'b. !f. compC (G (sharp [:'a,'b:] f)) eta = f)``,
+  STRIP_TAC
+  THEN IMP_RES_TAC g_adjf1_thm
+  THEN ASM_REWRITE_TAC []
+) ;
 
 val adjf1_conds_def = Define `adjf1_conds = \:'C 'D 'F 'G. 
-  \ (idC, compC) (idD,compD) eta F' G. 
+  \ (idC, compC) (idD,compD) eta (F': ('C,'D,'F) g_functor) 
+    (G : ('D,'C,'G) g_functor). 
   g_nattransf [:'C:] (idC, compC) (eta :!'a. ('a, 'a 'F 'G) 'C)
     (g_I [:'C:]) (G g_oo F') /\ 
   category [:'C:] (idC, compC) /\ 
@@ -171,14 +160,7 @@ val adjf1_conds_thm = store_thm ("adjf1_conds_thm",
       (eta :!'a. ('a, 'a 'F 'G) 'C) (g_I [:'C:]) (G g_oo F') /\ 
     category [:'C:] (idC, compC) /\ 
     g_functor [:'D, 'C, 'G:] (idD,compD) (idC,compC) G``,
-  EVERY [ REWRITE_TAC [adjf1_conds_def],
-    (CONV_TAC (REDEPTH_CONV
-      (REWR_CONV UNCURRY_DEF ORELSEC TY_BETA_CONV ORELSEC BETA_CONV))),
-    REFL_TAC ]) ;
-(*
-set_goal ([], tmhe) ;
-val (sgs, goal) = top_goal () ;
-*) 
+  SRW_TAC [] [adjf1_conds_def]) ;
 
 val g_adjf1D = tsfg (sfg (fst o EQ_IMP_RULE)) g_adjf1_thm ;
 val g_adjf1D1 = DISCH_ALL (tsfg (sfg (fst o EQ_IMP_RULE)) (UNDISCH g_adjf1D)) ; 
@@ -208,11 +190,13 @@ val ETA_def = Define
     (\:'e. flatt [:'e 'F, 'e:] idD) : ('C, I, 'F o 'G) g_nattransf` ;
 
 val EPS_thm = store_thm ("EPS_thm",
-  ``EPS [:'C, 'D:] (idC, compC) sharp = (\:'e. sharp [:'e 'G, 'e:] idC)``,
+  ``EPS [:'C, 'D:] (idC, compC) (sharp : ('C,'D, 'F,'G) g_sharp) =
+    (\:'e. sharp [:'e 'G, 'e:] idC)``,
   SRW_TAC [] [EPS_def]) ;
 
 val ETA_thm = store_thm ("ETA_thm",
-  ``ETA [:'D, 'C:] (idD, compD) flatt = (\:'e. flatt [:'e 'F, 'e:] idD)``,
+  ``ETA [:'D, 'C:] (idD, compD) (flatt : ('D,'C, 'G,'F) g_flatt) =
+    (\:'e. flatt [:'e 'F, 'e:] idD)``,
   SRW_TAC [] [ETA_def]) ;
 
 val FLATT_def = Define 
@@ -226,46 +210,42 @@ val SHARP_def = Define
     (\:'a 'b. \f : ('a, 'b 'G) 'C. compD eps (F' f)) : ('C,'D, 'F,'G) g_sharp`;
 
 val FLATT_thm = store_thm ("FLATT_thm", 
-  ``FLATT [:'D, 'C:] (idC, compC) G eta =
+  ``FLATT [:'D, 'C:] (idC, compC)
+          (G : ('D, 'C, 'G) g_functor) (eta : ('C, I, 'F o 'G) g_nattransf) =
     (\:'b 'a. \g : ('a 'F, 'b) 'D. compC (G g) eta)``,
   SRW_TAC [] [FLATT_def]) ;
 
 val SHARP_thm = store_thm ("SHARP_thm",  
-  ``SHARP [:'C, 'D:] (idD, compD) F' eps =
+  ``SHARP [:'C, 'D:] (idD, compD)
+          (F' : ('C, 'D, 'F) g_functor) (eps : ('D, 'G o 'F, I) g_nattransf) =
     (\:'a 'b. \f : ('a, 'b 'G) 'C. compD eps (F' f))``,
   SRW_TAC [] [SHARP_def]) ;
 
 (* parsing ETA_EPS_dual and SHARP_FLATT_dual requires _both_ type arguments *)
 
 val ETA_EPS_dual = store_thm ("ETA_EPS_dual",
-  ``(ETA [:'D, 'C:] ((idD, compD) : 'D category) flatt =
+  ``(ETA [:'D, 'C:] ((idD, compD) : 'D category)
+         (flatt : ('D,'C, 'G,'F) g_flatt) =
     (EPS [:'D C, 'C C:] (idD, dual_comp compD) flatt))``,
-  EVERY [ (REWRITE_TAC [ETA_thm, EPS_def]), TY_BETA_TAC,
-    (REWRITE_TAC [UNCURRY_DEF]), BETA_TAC, REFL_TAC ]) ;
+  SIMP_TAC bool_ss [ETA_thm, EPS_def, UNCURRY_DEF]) ;
 
 val EPS_ETA_dual = store_thm ("EPS_ETA_dual",
-  ``(EPS [:'C, 'D:] ((idC, compC) : 'C category) sharp =
+  ``(EPS [:'C, 'D:] ((idC, compC) : 'C category)
+         (sharp : ('C,'D, 'F,'G) g_sharp) =
     (ETA [:'C C, 'D C:] (idC, dual_comp compC) sharp))``,
-  EVERY [ (REWRITE_TAC [ETA_def, EPS_thm]), TY_BETA_TAC,
-    (REWRITE_TAC [UNCURRY_DEF]), BETA_TAC, REFL_TAC ]) ;
+  SIMP_TAC bool_ss [ETA_def, EPS_thm, UNCURRY_DEF]) ;
 
 val SHARP_FLATT_dual = store_thm ("SHARP_FLATT_dual",
-  ``SHARP [:'C, 'D:] (idD,compD) F' eps =
+  ``SHARP [:'C, 'D:] (idD,compD)
+          (F' : ('C, 'D, 'F) g_functor) (eps : ('D, 'G o 'F, I) g_nattransf) =
     FLATT [:'C C, 'D C:] (idD, dual_comp compD) (g_dual_functor F') eps``,
-  EVERY [
-    (REWRITE_TAC [SHARP_thm, FLATT_def, dual_comp_def, g_dual_functor_def]), 
-    (CONV_TAC (REDEPTH_CONV
-      (REWR_CONV UNCURRY_DEF ORELSEC TY_BETA_CONV ORELSEC BETA_CONV))),
-    REFL_TAC ]) ;
+  SIMP_TAC bool_ss [SHARP_thm, FLATT_def, dual_comp_def, g_dual_functor_def, UNCURRY_DEF]) ;
 
 val FLATT_SHARP_dual = store_thm ("FLATT_SHARP_dual",
-  ``FLATT [:'D, 'C:] (idC,compC) G eta =
+  ``FLATT [:'D, 'C:] (idC,compC)
+          (G : ('D, 'C, 'G) g_functor) (eta : ('C, I, 'F o 'G) g_nattransf) =
     SHARP [:'D C, 'C C:] (idC, dual_comp compC) (g_dual_functor G) eta``,
-  EVERY [
-    (REWRITE_TAC [SHARP_def, FLATT_thm, dual_comp_def, g_dual_functor_def]), 
-    (CONV_TAC (REDEPTH_CONV
-      (REWR_CONV UNCURRY_DEF ORELSEC TY_BETA_CONV ORELSEC BETA_CONV))),
-    REFL_TAC ]) ;
+  SIMP_TAC bool_ss [SHARP_def, FLATT_thm, dual_comp_def, g_dual_functor_def, UNCURRY_DEF]) ;
 
 val gatm =
 ``adjf1_conds [:'C, 'D, 'F, 'G:] (idC, compC) (idD,compD) eta F' G ==>
@@ -301,96 +281,77 @@ val tmhc =
     g_adjf1 (idC, compC) G eta sharp ==> 
     (sharp (compC g f) = compD (sharp g) (F' f))`` ;
 
-val g_adjf1_sharp_comp' = prove (tmhc,
-  EVERY [
-    (REWRITE_TAC [adjf1_conds_thm]), STRIP_TAC, 
-    (FIRST_ASSUM (MATCH_MP_TAC o MATCH_MP g_adjf1D1)),
-    (FIRST_X_ASSUM (fn th => REWRITE_TAC [MATCH_MP g_functorD th])),
-    (FIRST_ASSUM (fn th => REWRITE_TAC [MATCH_MP catDRAss th])),
-    (FIRST_X_ASSUM (fn th => REWRITE_TAC
-      [(REWRITE_RULE [o_THM, I_THM] o TY_BETA_RULE o REWRITE_RULE
-      [g_oo_thm, g_I_def] o MATCH_MP g_nattransfD) th])),
-    (FIRST_ASSUM (fn th => REWRITE_TAC [MATCH_MP categoryD th])),
-    (FIRST_X_ASSUM (fn th => REWRITE_TAC [MATCH_MP g_adjf1DGh th])) ]) ;
+val g_adjf1_sharp_comp = store_thm ("g_adjf1_sharp_comp", tmhc,
+  REWRITE_TAC [adjf1_conds_thm]
+  THEN STRIP_TAC
+  THEN FIRST_REP_RES MATCH_MP_TAC g_adjf1D1
+  THEN FIRST_REP_RES REWRITE_THM g_functorD
+  THEN FIRST_REP_RES REWRITE_THM catDRAss
+  THEN FIRST_REP_RES MP_TAC g_nattransfD
+  THEN SIMP_TAC combin_ss [g_oo_thm, g_I_def]
+  THEN DISCH_TAC
+  THEN FIRST_REP_RES REWRITE_THM categoryD
+  THEN FIRST_REP_RES REWRITE_THM g_adjf1DGh
+) ;
 
-val g_adjf1_sharp_comp = save_thm ("g_adjf1_sharp_comp",
-  DISCH_ALL (TY_GEN_ALL (GEN_ALL (UNDISCH g_adjf1_sharp_comp')))) ;
 
 val tmhe =
   ``adjf1_conds [:'C, 'D, 'F, 'G:] (idC, compC) (idD,compD) eta F' G /\
     g_adjf1 (idC, compC) G eta sharp ==> (compD (sharp idC) (F' f) = sharp f)`` ;
 
-val g_adjf1_sharp_eq' = prove (tmhe,
-  EVERY [ DISCH_TAC,
-    (FIRST_ASSUM (fn th => REWRITE_TAC [MATCH_MP (GSYM g_adjf1_sharp_comp) th])),
-    (POP_ASSUM (ASSUME_TAC o CONJUNCT1)),
-    (IMP_RES_TAC adjf1_conds_thm),
-    (FIRST_ASSUM (fn th => REWRITE_TAC [MATCH_MP catDLU th])) ]) ;
+val g_adjf1_sharp_eq = store_thm ("g_adjf1_sharp_eq", tmhe,
+  STRIP_TAC
+  THEN IMP_RES_TAC (GSYM g_adjf1_sharp_comp)
+  THEN ASM_REWRITE_TAC []
+  THEN IMP_RES_TAC adjf1_conds_thm
+  THEN IMP_RES_THEN REWRITE_THM catDLU
+) ;
 
-val g_adjf1_sharp_eq = save_thm ("g_adjf1_sharp_eq",
-  DISCH_ALL (TY_GEN_ALL (GEN_ALL (UNDISCH g_adjf1_sharp_eq')))) ;
 
-val g_adjf1_sharp_eta' = prove (
-  ``category (idC,compC) /\ g_functor (idD,compD) (idC,compC) G /\
-    g_adjf1 (idC, compC) G eta sharp ==> 
+val g_adjf1_sharp_eta = store_thm ("g_adjf1_sharp_eta", 
+  ``category (idC,compC) /\
+    g_functor (idD,compD) (idC,compC) (G : ('D, 'C, 'G) g_functor) /\
+    g_adjf1 (idC, compC) G
+            (eta : ('C, I, 'F o 'G) g_nattransf)
+            (sharp : ('C, 'D, 'F, 'G) g_sharp) ==> 
     (sharp [:'a, 'a 'F:] (eta [:'a:]) = idD [:'a 'F:])``,
-  EVERY [ STRIP_TAC,
-    (FIRST_ASSUM (MATCH_MP_TAC o MATCH_MP g_adjf1D1)),
-    (FIRST_X_ASSUM (fn th => REWRITE_TAC [MATCH_MP g_functorD th])),
-    (FIRST_X_ASSUM (MATCH_ACCEPT_TAC o MATCH_MP catDLU)) ]) ;
+  STRIP_TAC
+  THEN FIRST_REP_RES MATCH_MP_TAC g_adjf1D1
+  THEN FIRST_REP_RES REWRITE_THM g_functorD
+  THEN FIRST_REP_RES MATCH_ACCEPT_TAC catDLU
+) ;
 
-val g_adjf1_sharp_eta = save_thm ("g_adjf1_sharp_eta",
-  DISCH_ALL (TY_GEN_ALL (GEN_ALL (UNDISCH g_adjf1_sharp_eta')))) ;
 
 val tmfc = 
   ``adjf1_conds [:'C, 'D, 'F, 'G:] (idC, compC) (idD,compD) eta F' G /\
     category (idD, compD) /\ g_adjf1 (idC, compC) G eta sharp ==>
-    (F' f = sharp (compC eta f))`` ;
-  
-val g_adjf1_Feq' = prove (tmfc, 
-  EVERY [ STRIP_TAC,
-    (IMP_RES_TAC g_adjf1_sharp_comp),
-    (* (IMP_RES_TAC g_adjf1_sharp_comp') doesn't generalise over types *)
-    (IMP_RES_TAC adjf1_conds_thm),
-    (IMP_RES_TAC g_adjf1_sharp_eta),
-    (* (IMP_RES_TAC g_adjf1_sharp_eta') doesn't generalise over types *)
-    (ASM_REWRITE_TAC []),
-    (REPEAT (FIRST_X_ASSUM
-      (fn th => REWRITE_TAC [MATCH_MP catDLU th]))) ]) ;
+    (!:'a 'b. !f. F' [:'a,'b:] f = sharp (compC eta f))`` ;
 
-val g_adjf1_Feq = save_thm ("g_adjf1_Feq",
-  DISCH_ALL (TY_GEN_ALL (GEN_ALL (UNDISCH g_adjf1_Feq')))) ;
+val g_adjf1_Feq = store_thm ("g_adjf1_Feq", tmfc, 
+  STRIP_TAC
+  THEN IMP_RES_TAC g_adjf1_sharp_comp
+  THEN IMP_RES_TAC adjf1_conds_thm
+  THEN IMP_RES_TAC g_adjf1_sharp_eta
+  THEN ASM_REWRITE_TAC []
+  THEN IMP_RES_THEN REWRITE_THM catDLU
+) ;
 
-val g_adjf1_Feq_exp = (CONV_RULE (REDEPTH_CONV
-    (REWR_CONV UNCURRY_DEF ORELSEC TY_BETA_CONV ORELSEC BETA_CONV)))
-  (REWRITE_RULE [adjf1_conds_def] g_adjf1_Feq) ;
-val g_adjf1_Feq_exp' = 
-    (DISCH_ALL o SPEC_ALL o TY_SPEC_ALL o UNDISCH) g_adjf1_Feq_exp ;
+
+val g_adjf1_Feq_exp = SIMP_RULE bool_ss [UNCURRY_DEF,adjf1_conds_def] g_adjf1_Feq ;
 
 val tmfee = mk_imp 
   (list_mk_conj [catC, catD, funG, adjf1], mk_eq (Feq, nteta)) ;
 
-val g_adjf1_Feq_nt = store_thm ("g_adjf1_Feq_nt", tmfee, 
-  EVERY [ STRIP_TAC, EQ_TAC, STRIP_TAC] 
-  THENL [
-    EVERY [
-      (ASM_REWRITE_TAC [g_nattransf_thm, g_oo_thm, g_I_def]),
-      TY_BETA_TAC, (REWRITE_TAC [o_THM, I_THM]), BETA_TAC,
-      (REPEAT STRIP_TAC),
-      (FIRST_X_ASSUM (MATCH_ACCEPT_TAC o MATCH_MP g_adjf1DGh)) ],
-    EVERY [
-      (REWRITE_TAC [TY_FUN_EQ_THM, FUN_EQ_THM]),
-      (REPEAT STRIP_TAC), TY_BETA_TAC, BETA_TAC,
-      (MATCH_MP_TAC g_adjf1_Feq_exp'),
-      (ASM_REWRITE_TAC []) ]]) ;
-
-(*
-show_types := true ;
-show_types := false ;
-handle e => Raise e ;
-set_goal ([], it) ;
-val (sgs, goal) = top_goal () ;
-*)
+val g_adjf1_Feq_nt = store_thm ("g_adjf1_Feq_nt", tmfee,
+  STRIP_TAC THEN EQ_TAC THEN STRIP_TAC
+  THEN ASM_SIMP_TAC combin_ss [g_nattransf_thm, g_oo_thm, g_I_def]
+  THENL
+    [ IMP_RES_THEN MATCH_ACCEPT_TAC g_adjf1DGh,
+      SIMP_TAC bool_ss [TY_FUN_EQ_THM, FUN_EQ_THM]
+      THEN MATCH_MP_TAC g_adjf1_Feq_exp
+      THEN ASM_REWRITE_TAC []
+    ]
+) ;
 
 val tmff  =
 ``adjf1_conds [:'C, 'D, 'F, 'G:] (idC, compC) (idD,compD) eta F' G /\
@@ -398,42 +359,27 @@ val tmff  =
   g_functor (idC,compC) (idD,compD) F'`` ;
 
 val g_adjf1_F_fun = store_thm ("g_adjf1_F_fun", tmff,
-  EVERY [ DISCH_TAC,
-    (FIRST_ASSUM (ASSUME_TAC o MATCH_MP g_adjf1_Feq)),
-    (ASM_REWRITE_TAC [g_functor_thm]),
-    (POP_ASSUM_LIST (MAP_EVERY (MAP_EVERY ASSUME_TAC o CONJUNCTS))),
+  STRIP_TAC
+  THEN IMP_RES_TAC g_adjf1_Feq
+  THEN ASM_REWRITE_TAC [g_functor_thm]
     (* delete category (idD,compD) *)
-    (FIRST_X_ASSUM (fn th => (MATCH_MP categoryD th ; ALL_TAC))),
-    CONJ_TAC, (REPEAT STRIP_TAC),
-    (FIRST_ASSUM (MATCH_MP_TAC o MATCH_MP g_adjf1D1)),
-    (IMP_RES_TAC adjf1_conds_thm),
-    (FIRST_ASSUM (fn th => ASM_REWRITE_TAC [MATCH_MP g_functorD th])) ]
-  THENL [ (IMP_RES_TAC category_thm) THEN ASM_REWRITE_TAC [],
-    EVERY [ 
-      (FIRST_ASSUM (fn th => REWRITE_TAC [(MATCH_MP catDRAss th)])),
-      (FIRST_ASSUM (fn th => REWRITE_TAC [MATCH_MP g_adjf1DGh th])),
-      (FIRST_ASSUM (fn th => REWRITE_TAC [MATCH_MP catDAss th])),
-      (FIRST_ASSUM (fn th => REWRITE_TAC [MATCH_MP g_adjf1DGh th])) ]] ) ;
-
-(*
-show_types := true ;
-show_types := false ;
-handle e => Raise e ;
-set_goal ([], it) ;
-val (sgs, goal) = top_goal () ;
-*)
+  THEN FIRST_X_ASSUM (fn th => (MATCH_MP categoryD th ; ALL_TAC))
+  THEN REPEAT STRIP_TAC
+  THEN IMP_RES_THEN MATCH_MP_TAC g_adjf1D1
+  THEN MAP_EVERY IMP_RES_TAC [adjf1_conds_thm, g_functorD, category_thm]
+  THEN ASM_REWRITE_TAC []
+  THEN MAP_EVERY (FIRST_REP_RES REWRITE_THM)
+    [catDRAss,g_adjf1DGh,catDAss,g_adjf1DGh]
+);
 
 val sharp_flatt_inv_defs = store_thm ("sharp_flatt_inv_defs",
-  ``(category (idD,compD) /\ g_functor (idC,compC) (idD,compD) F' ==> 
-      (eps = EPS (idC,compC) (SHARP (idD,compD) F' eps))) /\ 
-    (category (idC,compC) /\ g_functor (idD,compD) (idC,compC) G ==> 
-      (eta = ETA (idD,compD) (FLATT (idC,compC) G eta)))``,
-  EVERY [ (REWRITE_TAC [SHARP_def, FLATT_def, EPS_thm, ETA_thm, 
-      g_functor_def, category_def]), 
-    (CONV_TAC (REDEPTH_CONV 
-      (REWR_CONV UNCURRY_DEF ORELSEC TY_BETA_CONV ORELSEC BETA_CONV))),
-    (REPEAT STRIP_TAC), (ASM_REWRITE_TAC []),
-    (CONV_TAC (ONCE_DEPTH_CONV TY_ETA_CONV)), REFL_TAC ] ) ;
+  ``(category (idD,compD) /\ g_functor [:'C,'D,'F:] (idC,compC) (idD,compD) F' ==> 
+      ((eps : ('D, 'G o 'F, I) g_nattransf) = EPS (idC,compC) (SHARP (idD,compD) F' eps))) /\ 
+    (category (idC,compC) /\ g_functor [:'D,'C,'G:] (idD,compD) (idC,compC) G ==> 
+      ((eta : ('C, I, 'F o 'G) g_nattransf) = ETA (idD,compD) (FLATT (idC,compC) G eta)))``,
+  SIMP_TAC (bool_ss ++ TY_ETA_ss)
+           [SHARP_def, FLATT_def, EPS_thm, ETA_thm, 
+            g_functor_def, category_def, UNCURRY_DEF] ) ;
 
 val [sharp_inv_def, flatt_inv_def] = CONJUNCTS sharp_flatt_inv_defs ;
 
@@ -441,12 +387,14 @@ val tmd = ``adjf1_conds [:'C, 'D, 'F, 'G:] (idC, compC) (idD,compD) eta F' G /\
   g_adjf1 (idC,compC) G eta sharp ==> 
   (sharp = SHARP (idD,compD) F' (EPS (idC,compC) sharp))`` ;
 
-val g_adjf1_IMP_defs = store_thm ("g_adjf1_IMP_defs", tmd, 
-  EVERY [ DISCH_TAC, MATCH_MP_TAC EQ_SYM,
-    (POP_ASSUM (ASSUME_TAC o MATCH_MP g_adjf1_sharp_eq)),
-    (SRW_TAC [] [SHARP_def, EPS_thm]),
-    (CONV_TAC (ONCE_DEPTH_CONV ETA_CONV)),
-    (CONV_TAC (TOP_DEPTH_CONV TY_ETA_CONV)), REFL_TAC ]) ;
+val g_adjf1_IMP_defs = store_thm ("g_adjf1_IMP_defs", tmd,
+  STRIP_TAC
+  THEN MATCH_MP_TAC EQ_SYM
+  THEN IMP_RES_TAC g_adjf1_sharp_eq
+  THEN SRW_TAC [] [SHARP_def, EPS_thm]
+  THEN CONV_TAC (TOP_DEPTH_CONV (ETA_CONV ORELSEC TY_ETA_CONV))
+  THEN REFL_TAC
+) ;
 
 val tment =
 ``adjf1_conds [:'C, 'D, 'F, 'G:] (idC, compC) (idD,compD) eta F' G /\
@@ -454,98 +402,81 @@ val tment =
   g_nattransf (idD,compD) (EPS (idC,compC) sharp) (F' g_oo G) (g_I [:'D:])`` ;
 
 val g_adjf1_eta_nt = store_thm ("g_adjf1_eta_nt", tment, 
-  EVERY [DISCH_TAC,
-    (REWRITE_TAC [g_nattransf_def, EPS_thm, g_oo_thm, g_I_def, o_DEF]),
-    (CONV_TAC (REDEPTH_CONV
-      (REWR_CONV UNCURRY_DEF ORELSEC TY_BETA_CONV ORELSEC BETA_CONV))),
-    (FIRST_ASSUM (fn th => 
-      ASM_REWRITE_TAC [I_THM, MATCH_MP g_adjf1_sharp_eq th])),
-    (POP_ASSUM (MAP_EVERY ASSUME_TAC o
-      CONJUNCTS o REWRITE_RULE [adjf1_conds_thm])),
-
-    (FIRST_ASSUM (ASSUME_TAC o MATCH_MP g_adjf1D1)),
-    (REPEAT STRIP_TAC), (MATCH_MP_TAC EQ_SYM),
-    (FIRST_X_ASSUM MATCH_MP_TAC),
-    
-    (FIRST_X_ASSUM (fn th => REWRITE_TAC [MATCH_MP g_functorD th])),
-    (FIRST_ASSUM (fn th => REWRITE_TAC [(MATCH_MP catDRAss th)])),
-    (FIRST_X_ASSUM (fn th => REWRITE_TAC [MATCH_MP g_adjf1DGh th])),
-    (FIRST_X_ASSUM (fn th => REWRITE_TAC [MATCH_MP catDRU th])) ]) ;
+  SRW_TAC [] [g_nattransf_def, EPS_thm, g_oo_thm, g_I_def, o_DEF]
+  THEN IMP_RES_TAC g_adjf1_sharp_eq
+  THEN ASM_REWRITE_TAC []
+  THEN IMP_RES_TAC adjf1_conds_thm
+  THEN FIRST_REP_RES (MATCH_MP_TAC o GSYM) g_adjf1D1
+  THEN MAP_EVERY (FIRST_REP_RES REWRITE_THM) 
+    [g_functorD,catDRAss,g_adjf1DGh,catDRU]
+) ;
 
 val tm13 = ``adjf1_conds [:'C, 'D, 'F, 'G:] (idC, compC) (idD,compD) eta F' G /\
        g_adjf1 (idC, compC) G eta sharp ==> 
        g_adjf3 (idC, compC) (idD,compD) F' G eta (EPS (idC, compC) sharp)`` ;
 
 val g_adjf1_3 = store_thm ("g_adjf1_3", tm13,
-  EVERY [ (REWRITE_TAC [g_adjf3_thm, EPS_thm]), DISCH_TAC, TY_BETA_TAC,
-    (FIRST_ASSUM (MAP_EVERY ASSUME_TAC o CONJUNCTS)),
-    (FIRST_X_ASSUM (fn th => REWRITE_TAC [MATCH_MP g_adjf1_sharp_eq th])),
-    (FIRST_X_ASSUM (fn th => REWRITE_TAC [MATCH_MP g_adjf1D th])) ]) ;
-
-(*
-show_types := true ;
-show_types := false ;
-handle e => Raise e ;
-set_goal ([], it) ;
-val (sgs, goal) = top_goal () ;
-*)
+  SIMP_TAC satisfy_ss [g_adjf3_thm, EPS_thm, g_adjf1_sharp_eq, g_adjf1D]) ;
 
 (* prove g_adjf2_3 by duality from g_adjf1_3 *)
-val tm23 = ``g_nattransf (idD,compD) eps (F' g_oo G) (g_I [:'D:]) /\
+val tm23 = ``g_nattransf (idD,compD) (eps : ('D, 'G o 'F, I) g_nattransf)
+                         ((F':('C, 'D, 'F) g_functor) g_oo (G:('D, 'C, 'G) g_functor))
+                         (g_I [:'D:]) /\
        category (idD,compD) /\ g_functor (idC,compC) (idD,compD) F' /\
        g_adjf2 (idD, compD) F' eps flatt ==> 
        g_adjf3 (idC, compC) (idD,compD) F' G (ETA (idD, compD) flatt) eps`` ;
 
 val g_adjf2_3 = store_thm ("g_adjf2_3", tm23,
-  EVERY [ (REWRITE_TAC [g_adjf12_dual]), (STRIP_TAC),
-    (CONV_TAC (REWR_CONV g_adjf3_dual)),
-    (REWRITE_TAC [ETA_EPS_dual]),
-    (MATCH_MP_TAC g_adjf1_3), 
-    (REWRITE_TAC [adjf1_conds_def]),
-    (CONV_TAC (REDEPTH_CONV
-      (REWR_CONV UNCURRY_DEF ORELSEC TY_BETA_CONV ORELSEC BETA_CONV))),
-    (ASM_REWRITE_TAC (map GSYM [g_functor_dual, category_dual])),
-    (FIRST_X_ASSUM (ASSUME_TAC o 
-      MATCH_MP (fst (EQ_IMP_RULE g_nattransf_dual)))),
-    (FIRST_ASSUM (ACCEPT_TAC o REWRITE_RULE [g_I_dual, g_oo_dual])) ]) ;
+  REWRITE_TAC [g_adjf12_dual]
+  THEN STRIP_TAC
+  THEN CONV_TAC (REWR_CONV g_adjf3_dual)
+  THEN REWRITE_TAC [ETA_EPS_dual]
+  THEN MATCH_MP_TAC g_adjf1_3
+  THEN ASM_SIMP_TAC bool_ss [adjf1_conds_def,UNCURRY_DEF,
+                             GSYM g_functor_dual,GSYM category_dual]
+  THEN IMP_RES_THEN MP_TAC g_nattransf_dual
+  THEN REWRITE_TAC [g_I_dual, g_oo_dual]
+) ;
 
 val g_adjf3_1 = store_thm ("g_adjf3_1",
-  ``g_adjf3 (idC, compC) (idD,compD) F' G eta eps =
+  ``g_adjf3 [:'C,'D, 'F,'G:] (idC, compC) (idD,compD) F' G eta eps =
     g_adjf1 (idC, compC) G eta (SHARP (idD,compD) F' eps)``,
-  EVERY [ (REWRITE_TAC [g_adjf3_thm, g_adjf1_thm, SHARP_def]),
-    (CONV_TAC (REDEPTH_CONV
-      (REWR_CONV UNCURRY_DEF ORELSEC TY_BETA_CONV ORELSEC BETA_CONV))),
-    REFL_TAC] ) ;
+  SIMP_TAC bool_ss [g_adjf3_thm, g_adjf1_thm, SHARP_def, UNCURRY_DEF]
+) ;
 
 val g_adjf3_2 = store_thm ("g_adjf3_2",
-  ``g_adjf3 (idC, compC) (idD,compD) F' G eta eps =
+  ``g_adjf3 (idC, compC) (idD,compD)
+            (F':('C, 'D, 'F) g_functor) (G:('D, 'C, 'G) g_functor) eta eps =
     g_adjf2 (idD,compD) F' eps (FLATT (idC, compC) G eta)``,
-  EVERY [ (REWRITE_TAC [g_adjf3_thm, g_adjf2_thm, FLATT_def]),
-    (CONV_TAC (REDEPTH_CONV
-      (REWR_CONV UNCURRY_DEF ORELSEC TY_BETA_CONV ORELSEC BETA_CONV))),
-    EQ_TAC, DISCH_TAC, ASM_REWRITE_TAC [] ] ) ;
+  SIMP_TAC bool_ss [g_adjf3_thm, g_adjf2_thm, FLATT_def, UNCURRY_DEF]
+  THEN EQ_TAC THEN DISCH_THEN REWRITE_THM
+) ;
 
 val g_adjf1_2 = save_thm ("g_adjf1_2", REWRITE_RULE [g_adjf3_2] g_adjf1_3) ;
 
 val SHARP_eta_I = store_thm ("SHARP_eta_I", 
-  ``g_adjf3 (idC,compC) (idD,compD) F' G (eta : ('C, I, 'F o 'G) g_nattransf)
-      (eps : ('D, 'G o 'F, I) g_nattransf) /\
+  ``g_adjf3 (idC,compC) (idD,compD)
+            (F':('C, 'D, 'F) g_functor) (G:('D, 'C, 'G) g_functor)
+            (eta : ('C, I, 'F o 'G) g_nattransf)
+            (eps : ('D, 'G o 'F, I) g_nattransf) /\
     category (idC, compC) /\ g_functor (idD,compD) (idC,compC) G ==> 
     (compD eps (F' eta) = idD)``,
-  EVERY [ STRIP_TAC,
-    (FIRST_X_ASSUM (MATCH_MP_TAC o MATCH_MP g_adjf3D1)),
-    (FIRST_X_ASSUM (fn th => REWRITE_TAC [MATCH_MP g_functorD th])),
-    (FIRST_X_ASSUM (MATCH_ACCEPT_TAC o MATCH_MP catDLU)) ]) ;
+  STRIP_TAC
+  THEN FIRST_REP_RES MATCH_MP_TAC g_adjf3D1
+  THEN MAP_EVERY (FIRST_REP_RES REWRITE_THM) [g_functorD,catDLU]
+) ;
 
 val FLATT_eps_I = store_thm ("FLATT_eps_I", 
-  ``g_adjf3 (idC,compC) (idD,compD) F' G (eta : ('C, I, 'F o 'G) g_nattransf)
-      (eps : ('D, 'G o 'F, I) g_nattransf) /\
+  ``g_adjf3 (idC,compC) (idD,compD)
+            (F':('C, 'D, 'F) g_functor) (G:('D, 'C, 'G) g_functor)
+            (eta : ('C, I, 'F o 'G) g_nattransf)
+            (eps : ('D, 'G o 'F, I) g_nattransf) /\
     category (idD, compD) /\ g_functor (idC,compC) (idD,compD) F' ==>
     (compC (G eps) eta = idC)``,
-  EVERY [ STRIP_TAC,
-    (FIRST_X_ASSUM (MATCH_MP_TAC o MATCH_MP g_adjf3D2)),
-    (FIRST_X_ASSUM (fn th => REWRITE_TAC [MATCH_MP g_functorD th])),
-    (FIRST_X_ASSUM (MATCH_ACCEPT_TAC o MATCH_MP catDRU)) ]) ;
+  STRIP_TAC
+  THEN FIRST_REP_RES MATCH_MP_TAC g_adjf3D2
+  THEN MAP_EVERY (FIRST_REP_RES REWRITE_THM) [g_functorD,catDRU]
+) ;
 
 (* this is the actual formulation of the equivalence of two
   characterisations of adjoint functors *)
@@ -559,38 +490,50 @@ val tm13e = mk_imp (list_mk_conj [catC, catD, funG, nteta],
   mk_eq (mk_conj (adjf1, eps), list_mk_conj [adjf3, funF, nteps, sharp])) ;
 
 val g_adjf13_equiv = store_thm ("g_adjf13_equiv", tm13e,
-  (STRIP_TAC THEN EQ_TAC THEN STRIP_TAC) THENL [
-    (EVERY [ (REPEAT CONJ_TAC), (ASM_REWRITE_TAC []),
-      (FIRST (map (MATCH_MP_TAC o REWRITE_RULE [adjf1_conds_def]) 
-	[ g_adjf1_3, g_adjf1_F_fun, g_adjf1_eta_nt, g_adjf1_IMP_defs ])),
-      (CONV_TAC (REDEPTH_CONV
-	  (REWR_CONV UNCURRY_DEF ORELSEC TY_BETA_CONV ORELSEC BETA_CONV))),
-      (ASM_REWRITE_TAC []) ] ),
-    (EVERY [ (REPEAT CONJ_TAC), (ASM_REWRITE_TAC []),
-      (MATCH_MP_TAC (fst (EQ_IMP_RULE g_adjf3_1)) ORELSE
-	MATCH_MP_TAC (CONJUNCT1 sharp_flatt_inv_defs)),
-      (ASM_REWRITE_TAC []) ]) ]) ;
+  STRIP_TAC
+  THEN EQ_TAC
+  THEN STRIP_TAC
+  THENL
+    [ REPEAT CONJ_TAC
+      THEN ASM_REWRITE_TAC []
+      THENL
+        [ MATCH_MP_TAC g_adjf1_3,
+          MATCH_MP_TAC g_adjf1_F_fun,
+          MATCH_MP_TAC g_adjf1_eta_nt,
+          MATCH_MP_TAC g_adjf1_IMP_defs
+        ]
+      THEN ASM_SIMP_TAC bool_ss [UNCURRY_DEF,adjf1_conds_def],
+
+      REPEAT CONJ_TAC
+      THEN ASM_REWRITE_TAC []
+      THENL
+        [ ASM_REWRITE_TAC [GSYM g_adjf3_1],
+          IMP_RES_TAC (GSYM sharp_flatt_inv_defs)
+          THEN ASM_REWRITE_TAC []
+        ]
+    ]
+) ;
 
 (* get directly from g_adjf3 /\ F',G functors that eps and eta are nts *)
 val tm3nt = mk_imp (list_mk_conj [adjf3, catC, catD, funF, funG],
   mk_conj (nteta, nteps)) ;
 
-val g_adjf3_nt = store_thm ("g_adjf3_nt", tm3nt, 
-  EVERY [ STRIP_TAC, (IMP_RES_TAC g_functorD),
-    (IMP_RES_TAC catDLU), (IMP_RES_TAC catDRU),
-    (SRW_TAC [] [g_nattransf_def, g_oo_def, g_I_def]) ]
-  THENL [
-    EVERY [
-      (FIRST_ASSUM (MATCH_MP_TAC o MATCH_MP g_adjf3D2)),
-      (ASM_REWRITE_TAC []),
-      (FIRST_ASSUM (fn th => CHANGED_TAC (REWRITE_TAC [MATCH_MP catDAss th]))),
-      (USE_LIM_RES_TAC (fn th => ASM_REWRITE_TAC [th]) (SHARP_eta_I))],
-    EVERY [
-      (FIRST_ASSUM (MATCH_MP_TAC o GSYM o MATCH_MP g_adjf3D1)),
-      (ASM_REWRITE_TAC []),
-      (FIRST_ASSUM (fn th => CHANGED_TAC 
-	(REWRITE_TAC [MATCH_MP catDRAss th]))),
-      (USE_LIM_RES_TAC (fn th => ASM_REWRITE_TAC [th]) ( FLATT_eps_I))]] ) ;
+val g_adjf3_nt = store_thm ("g_adjf3_nt", tm3nt,
+  STRIP_TAC
+  THEN MAP_EVERY IMP_RES_TAC [g_functorD, catDLU, catDRU]
+  THEN SRW_TAC [] [g_nattransf_def, g_oo_def, g_I_def]
+  THENL
+    [ FIRST_REP_RES MATCH_MP_TAC g_adjf3D2
+      THEN ASM_REWRITE_TAC []
+      THEN IMP_RES_THEN REWRITE_THM catDAss
+      THEN FIRST_REP_RES_MKI ASM_REWRITE_THM SHARP_eta_I,
+
+      FIRST_REP_RES MATCH_MP_TAC (GSYM g_adjf3D1)
+      THEN ASM_REWRITE_TAC []
+      THEN IMP_RES_THEN REWRITE_THM catDRAss
+      THEN FIRST_REP_RES_MKI ASM_REWRITE_THM FLATT_eps_I
+    ]
+) ;
      
 val dual_convs = 
   [g_adjf3_dual, g_adjf12_dual, ETA_EPS_dual, EPS_ETA_dual, 
@@ -603,10 +546,8 @@ val tm23e = mk_imp (list_mk_conj [catD, catC, funF, nteps],
   mk_eq (mk_conj (adjf2, eta), list_mk_conj [adjf3, funG, nteta, flatt])) ;
 
 val g_adjf23_equiv = store_thm ("g_adjf23_equiv", tm23e,
-  EVERY [
-    (CONV_TAC (ONCE_DEPTH_CONV (FIRST_CONV (map REWR_CONV dual_convs)))),
-    (REWRITE_TAC [g_oo_dual, g_I_dual]),
-    (MATCH_ACCEPT_TAC g_adjf13_equiv) ]) ;
+  ONCE_REWRITE_TAC dual_convs
+  THEN SIMP_TAC bool_ss [g_oo_dual, g_I_dual, g_adjf13_equiv]) ;
 
 val tm12e = mk_imp (mk_conj (catC, catD),
   mk_eq (list_mk_conj [adjf1, funG, nteta, eps, flatt],
@@ -625,147 +566,138 @@ val [ga13', ga31', ga23', ga32'] =
 fun usega th = (CHANGED_TAC (REWRITE_TAC [th]) THEN
   MAP_EVERY ASSUME_TAC (CONJUNCTS th)) ;
 
-val g_adjf12_equiv = store_thm ("g_adjf12_equiv", tm12e,
-  EVERY [ STRIP_TAC, EQ_TAC, STRIP_TAC ]
-  THENL [ FIRST_REP_RES_MKI usega ga13' THEN FIRST_REP_RES_MKI usega ga32',
-    FIRST_REP_RES_MKI usega ga23' THEN FIRST_REP_RES_MKI usega ga31' ]) ;
+fun usega th = (CHANGED_TAC (REWRITE_TAC [th]) THEN
+  STRIP_ASSUME_TAC th) ;
 
-val seith = DISCH_ALL (TY_GEN_ALL (UNDISCH FLATT_eps_I)) ;
-val heith = DISCH_ALL (TY_GEN_ALL (UNDISCH SHARP_eta_I)) ;
+val g_adjf12_equiv = store_thm ("g_adjf12_equiv", tm12e,
+  STRIP_TAC
+  THEN EQ_TAC
+  THEN STRIP_TAC
+  THENL
+    [ FIRST_REP_RES_MKI usega ga13' THEN FIRST_REP_RES_MKI usega ga32',
+      FIRST_REP_RES_MKI usega ga23' THEN FIRST_REP_RES_MKI usega ga31' ]) ;
 
 val tm43 = mk_imp (list_mk_conj [adjf4, catC, catD, eta, eps, Feq, Geq],
   list_mk_conj [funF, funG, nteta, nteps, adjf3, sharp, flatt]) ;
 
 val g_adjf4_3 = store_thm ("g_adjf4_3", tm43,
-  EVERY [ STRIP_TAC, (IMP_RES_TAC catDLU), (IMP_RES_TAC catDRU),
-    (SRW_TAC [] [g_adjf3_thm, ETA_thm, EPS_thm, SHARP_thm, FLATT_thm,
-      g_functor_thm, g_nattransf_thm]) ]
+  STRIP_TAC
+  THEN MAP_EVERY IMP_RES_TAC [catDLU,catDRU]
+  THEN SRW_TAC [] [g_adjf3_thm, ETA_thm, EPS_thm, SHARP_thm, FLATT_thm,
+                   g_functor_thm, g_nattransf_thm]
   THENL [
     (* F' and G functors *)
-    (FIRST_ASSUM (MATCH_MP_TAC o MATCH_MP g_adjf4D_eqv1)) THEN REFL_TAC,
+    IMP_RES_THEN MATCH_MP_TAC g_adjf4D_eqv1 THEN REFL_TAC,
 
-    (FIRST_ASSUM (fn th => REWRITE_TAC [GSYM (MATCH_MP g_adjf4D_sharp th)])) 
-      THEN (REPEAT 
-        (FIRST_X_ASSUM (fn th => REWRITE_TAC [MATCH_MP catDAss th]))),
+    IMP_RES_THEN (REWRITE_THM o GSYM) g_adjf4D_sharp
+    THEN IMP_RES_THEN REWRITE_THM catDAss,
 
-    (FIRST_ASSUM (MATCH_MP_TAC o MATCH_MP g_adjf4D_eqv2)) THEN REFL_TAC,
+    IMP_RES_THEN MATCH_MP_TAC g_adjf4D_eqv2 THEN REFL_TAC,
 
-    (FIRST_ASSUM (fn th => REWRITE_TAC [GSYM (MATCH_MP g_adjf4D_flatt th)]))
-      THEN (REPEAT
-        (FIRST_X_ASSUM (fn th => REWRITE_TAC [MATCH_MP catDAss th]))),
+    IMP_RES_THEN (REWRITE_THM o GSYM) g_adjf4D_flatt
+    THEN IMP_RES_THEN REWRITE_THM catDAss,
 
     (* eta and eps are natural transformations *)
     (*
-    e (REWRITE_TAC [g_oo_def, o_DEF]) ; (* does nothing - why ?? *)
+    e (REWRITE_TAC [g_oo_def, o_DEF]) ; (* does nothing - why ?? *) (* PVH: Now it does *)
     *)
-    EVERY [ (REWRITE_TAC [g_oo_def]), (* has an effect *)
-      (SRW_TAC [] [o_THM, g_I_def]),
-      (FIRST_ASSUM (fn th => 
-	ASM_REWRITE_TAC [GSYM (MATCH_MP g_adjf4D_flatt th)])),
-      (FIRST_ASSUM (MATCH_MP_TAC o MATCH_MP g_adjf4D_eqv2)), REFL_TAC],
+    ASM_SIMP_TAC combin_ss [g_oo_def, g_I_def]
+    THEN IMP_RES_THEN (fn th => ASM_REWRITE_TAC[GSYM th]) g_adjf4D_flatt
+    THEN IMP_RES_THEN MATCH_MP_TAC g_adjf4D_eqv2 THEN REFL_TAC,
 
-    EVERY [ (REWRITE_TAC [g_oo_def, g_I_def]), (* has an effect *)
-      (SRW_TAC [] [o_THM]),
-      (FIRST_ASSUM (fn th => 
-	ASM_REWRITE_TAC [GSYM (MATCH_MP g_adjf4D_sharp th)])),
-      (FIRST_ASSUM (MATCH_MP_TAC o GSYM o MATCH_MP g_adjf4D_eqv1)), REFL_TAC],
+    ASM_SIMP_TAC combin_ss [g_oo_def, g_I_def]
+    THEN IMP_RES_THEN (fn th => ASM_REWRITE_TAC[GSYM th]) g_adjf4D_sharp
+    THEN IMP_RES_THEN (MATCH_MP_TAC o GSYM) g_adjf4D_eqv1 THEN REFL_TAC,
 
     (* finally, the equivalence condition, g_adjf3 *)
-    EVERY [
-      (FIRST_ASSUM (fn th => REWRITE_TAC [GSYM (MATCH_MP g_adjf4D_flatt th)])),
-      (FIRST_ASSUM (fn th => 
-	ASM_REWRITE_TAC [GSYM (MATCH_MP g_adjf4D_sharp th)])),
-      (FIRST_ASSUM (MATCH_ACCEPT_TAC o MATCH_MP g_adjf4D_eqv))],
+    IMP_RES_THEN (REWRITE_THM o GSYM) g_adjf4D_flatt
+    THEN IMP_RES_THEN (fn th => ASM_REWRITE_TAC[GSYM th]) g_adjf4D_sharp
+    THEN IMP_RES_THEN MATCH_ACCEPT_TAC g_adjf4D_eqv,
 
-    EVERY [ (FIRST_ASSUM
-        (fn th => ASM_REWRITE_TAC [GSYM (MATCH_MP g_adjf4D_sharp th)])),
-      (CONV_TAC (DEPTH_CONV ETA_CONV)),
-      (CONV_TAC (DEPTH_CONV TY_ETA_CONV)), REFL_TAC],
+    IMP_RES_THEN (fn th => ASM_REWRITE_TAC[GSYM th]) g_adjf4D_sharp
+    THEN CONV_TAC (DEPTH_CONV (ETA_CONV ORELSEC TY_ETA_CONV))
+    THEN REFL_TAC,
 
-    EVERY [ (FIRST_ASSUM
-        (fn th => ASM_REWRITE_TAC [GSYM (MATCH_MP g_adjf4D_flatt th)])),
-      (CONV_TAC (DEPTH_CONV ETA_CONV)),
-      (CONV_TAC (DEPTH_CONV TY_ETA_CONV)), REFL_TAC] ]) ;
+    IMP_RES_THEN (fn th => ASM_REWRITE_TAC[GSYM th]) g_adjf4D_flatt
+    THEN CONV_TAC (DEPTH_CONV (ETA_CONV ORELSEC TY_ETA_CONV))
+    THEN REFL_TAC ]) ;
 
-(*
-show_types := true ;
-show_types := false ;
-handle e => Raise e ;
-set_goal ([], it) ;
-val (sgs, goal) = top_goal () ;
-*)
-val tm34 = ``g_adjf3 [:'C,'D:] (idC,compC) (idD,compD) F' G eta eps /\
-  category (idC,compC) /\ category (idD,compD) /\ 
+val tm34 =
+``g_adjf3 [:'C,'D:] (idC,compC) (idD,compD)
+                     (F':('C, 'D, 'F) g_functor) (G:('D, 'C, 'G) g_functor)
+                     eta eps /\
+       category (idC,compC) /\ category (idD,compD) /\ 
        g_functor (idC,compC) (idD,compD) F' /\
        g_functor (idD,compD) (idC,compC) G ==>
   g_adjf4 [:'C, 'D:] (idC,compC) (idD,compD) 
     (SHARP (idD,compD) F' eps) (FLATT (idC, compC) G eta)`` ;
 
-val g_adjf3_4 = store_thm ("g_adjf3_4", tm34, 
-  EVERY [ STRIP_TAC,
-    (USE_LIM_RES_TAC ASSUME_TAC ( heith)),
-    (USE_LIM_RES_TAC ASSUME_TAC ( seith)),
-    (SRW_TAC [] [g_adjf4_thm, SHARP_thm, FLATT_thm]),
-    (IMP_RES_TAC g_functor_thm),
-    (IMP_RES_TAC catDLU), (IMP_RES_TAC catDRU) ] 
-  THENL [
-    (FIRST_X_ASSUM (MATCH_ACCEPT_TAC o MATCH_MP g_adjf3D)),
-    EVERY [ (ASM_REWRITE_TAC []),
-      (FIRST_ASSUM (fn th => 
-	CHANGED_TAC (REWRITE_TAC [MATCH_MP catDRAss th]))),
-      (REPEAT (AP_THM_TAC ORELSE AP_TERM_TAC)),
-      (FIRST_ASSUM (fn th => 
-	CHANGED_TAC (ASM_REWRITE_TAC [MATCH_MP catDAss th]))) ],
-    EVERY [ (ASM_REWRITE_TAC []),
-      (FIRST_ASSUM (fn th => 
-	CHANGED_TAC (REWRITE_TAC [MATCH_MP catDAss th]))),
-      (REPEAT (AP_THM_TAC ORELSE AP_TERM_TAC)),
-      (FIRST_ASSUM (fn th => 
-	CHANGED_TAC (ASM_REWRITE_TAC [MATCH_MP catDRAss th]))) ]]) ;
+val g_adjf3_4 = store_thm ("g_adjf3_4", tm34,
+  STRIP_TAC
+  THEN IMP_RES_TAC (REWRITE_RULE[GSYM AND_IMP_INTRO] SHARP_eta_I)
+  THEN IMP_RES_TAC (REWRITE_RULE[GSYM AND_IMP_INTRO] FLATT_eps_I)
+  THEN MAP_EVERY IMP_RES_TAC [g_functor_thm,catDLU,catDRU]
+  THEN SRW_TAC [] [g_adjf4_thm, SHARP_thm, FLATT_thm]
+  THENL (* 3 subgoals *)
+    [ IMP_RES_THEN MATCH_ACCEPT_TAC g_adjf3D,
+
+      IMP_RES_THEN REWRITE_THM catDRAss
+      THEN REPEAT (AP_THM_TAC ORELSE AP_TERM_TAC)
+      THEN IMP_RES_THEN ASM_REWRITE_THM catDAss,
+
+      IMP_RES_THEN REWRITE_THM catDAss
+      THEN REPEAT (AP_THM_TAC ORELSE AP_TERM_TAC)
+      THEN IMP_RES_THEN ASM_REWRITE_THM catDRAss
+    ]) ;
 
 val tm34e = ``category (idC,compC) /\ category (idD,compD) ==> 
-  (g_adjf3 [:'C,'D:] (idC,compC) (idD,compD) F' G eta eps /\
+  (g_adjf3 [:'C,'D:] (idC,compC) (idD,compD)
+                     (F':('C, 'D, 'F) g_functor) (G:('D, 'C, 'G) g_functor)
+           eta eps /\
     g_functor (idC,compC) (idD,compD) F' /\
     g_functor (idD,compD) (idC,compC) G /\
     (sharp = SHARP (idD,compD) F' eps) /\ (flatt = FLATT (idC, compC) G eta) =
   g_adjf4 [:'C, 'D:] (idC,compC) (idD,compD) sharp flatt /\
     (eta = ETA (idD,compD) flatt) /\ (eps = EPS (idC,compC) sharp) /\
     (F' = (\:'a 'b. (\f. sharp (compC eta f)))) /\
-    (G = (\:'a 'b. (\g. flatt (compD g eps))))) `` ; 
+    (G = (\:'a 'b. (\g. flatt (compD g eps))))) `` ;
 
-val g_adjf34_equiv = store_thm ("g_adjf34_equiv", tm34e, 
-  EVERY [ STRIP_TAC, EQ_TAC, STRIP_TAC ] 
-    THENL [
-      EVERY [
-	(USE_LIM_RES_TAC ASSUME_TAC ( g_adjf3_4)),
-	(ASM_REWRITE_TAC []), (IMP_RES_TAC g_functorD),
-	(IMP_RES_TAC catDLU), (IMP_RES_TAC catDRU),
-	(REPEAT CONJ_TAC) ]
-      THENL [ (MATCH_MP_TAC flatt_inv_def) THEN (ASM_REWRITE_TAC []),
-	(MATCH_MP_TAC sharp_inv_def) THEN (ASM_REWRITE_TAC []),
+val g_adjf34_equiv = store_thm ("g_adjf34_equiv", tm34e,
+  STRIP_TAC
+  THEN EQ_TAC
+  THEN STRIP_TAC
+  THENL
+    [ IMP_RES_TAC (REWRITE_RULE[GSYM AND_IMP_INTRO] g_adjf3_4)
+      THEN ASM_REWRITE_TAC []
+      THEN MAP_EVERY IMP_RES_TAC [g_functorD,catDLU,catDRU]
+      THEN REPEAT CONJ_TAC
+      THENL (* 4 subgoals *)
+        [ MATCH_MP_TAC flatt_inv_def THEN ASM_REWRITE_TAC [],
 
-	EVERY [ (SRW_TAC [] [SHARP_thm]),
-	  (FIRST_ASSUM (fn th =>
-	    CHANGED_TAC (REWRITE_TAC [MATCH_MP catDAss th]))),
-	  (USE_LIM_RES_TAC (fn th => ASM_REWRITE_TAC [th]) ( SHARP_eta_I)),
-	  (CONV_TAC (DEPTH_CONV ETA_CONV)),
-	  (CONV_TAC (DEPTH_CONV TY_ETA_CONV)), REFL_TAC],
-	
-	EVERY [ (SRW_TAC [] [FLATT_thm]),
-	  (FIRST_ASSUM (fn th =>
-	    CHANGED_TAC (REWRITE_TAC [MATCH_MP catDRAss th]))),
-	  (USE_LIM_RES_TAC (fn th => ASM_REWRITE_TAC [th]) ( FLATT_eps_I)),
-	  (CONV_TAC (DEPTH_CONV ETA_CONV)),
-	  (CONV_TAC (DEPTH_CONV TY_ETA_CONV)), REFL_TAC] ],
+          MATCH_MP_TAC sharp_inv_def THEN ASM_REWRITE_TAC [],
 
-      (USE_LIM_RES_TAC (fn th => REWRITE_TAC [th]) ( g_adjf4_3)) ]) ;
-	
+          SRW_TAC [] [SHARP_thm]
+          THEN IMP_RES_THEN REWRITE_THM catDAss
+          THEN USE_LIM_RES_TAC ASM_REWRITE_THM SHARP_eta_I
+          THEN CONV_TAC (DEPTH_CONV (ETA_CONV ORELSEC TY_ETA_CONV))
+          THEN REFL_TAC,
+
+          SRW_TAC [] [FLATT_thm]
+          THEN IMP_RES_THEN REWRITE_THM catDRAss
+          THEN USE_LIM_RES_TAC ASM_REWRITE_THM FLATT_eps_I
+          THEN CONV_TAC (DEPTH_CONV (ETA_CONV ORELSEC TY_ETA_CONV))
+          THEN REFL_TAC
+        ],
+
+      USE_LIM_RES_TAC REWRITE_THM g_adjf4_3
+    ]) ;
+
 (* observe that from g_adjf4 we prove that eta and eps are nts,
   but we don't use this to get back to g_adjf4 from g_adjf3 ;
   thus it follows that g_adjf3 implies that eta and eps are nts,
   which is proved directly in g_adjf3nt *) 
 
-(* type-checking this fails, with a very strange message, namely 
+(* type-checking this fails (* PVH: now it works *), with a very strange message, namely 
 Type inference failure: unable to infer a type for the application of
 
 $= (F' :∀α β. (α, β) ('C: ar 2) -> (α ('F: ar 1), β 'F) ('D: ar 2))
@@ -788,9 +720,11 @@ which has type
 
 
 val tm14e = ``category (idC,compC) ∧ category (idD,compD) ==>
-  (g_adjf1 [:'C,'D:] (idC,compC) G eta sharp /\
+  (g_adjf1 [:'C,'D, 'F,'G:] (idC,compC) G
+                     (eta : ('C, I, 'F o 'G) g_nattransf) sharp /\
     g_functor (idD,compD) (idC,compC) G /\
-    g_nattransf [:'C:] (idC, compC) eta (g_I [:'C:]) (G g_oo F') /\ 
+    g_nattransf [:'C:] (idC, compC) eta (g_I [:'C:])
+                       (G g_oo (F' : ('C, 'D, 'F) g_functor)) /\ 
     (flatt = FLATT (idC, compC) G eta) = 
   g_adjf4 [:'C,'D:] (idC,compC) (idD,compD) sharp flatt /\
     (eta = ETA (idD,compD) flatt) /\ (eps = EPS (idC,compC) sharp) /\
@@ -799,7 +733,8 @@ val tm14e = ``category (idC,compC) ∧ category (idD,compD) ==>
 
 *)
 
-(* there must be an easier way than this !! *)
+(* there must be an easier way than this !! *) (* PVH: trying another way after this *)
+(*
 local val (th0, _) = EQ_IMP_RULE (UNDISCH g_adjf13_equiv) ;
 val th1 = REWRITE_RULE [GSYM AND_IMP_INTRO] th0 ;
 val (eps, EPS) = dest_eq (lhand (concl (UNDISCH th1))) ;
@@ -829,35 +764,55 @@ val (a1, th0) = (UNDISCH_TERM g_adjf13_equiv) ;
 val (_, g31D) = EQ_IMP_RULE th0 ;
 val g_adjf3_eq1 = REWRITE_RULE [GSYM AND_IMP_INTRO]
   (DISCH_ALL (DISCH a1 (UNDISCH g31D))) ;
-
+*)
 
 val tm14e = ``category (idC,compC) /\ category (idD,compD) ==>
-  (g_adjf1 [:'C,'D:] (idC,compC) G eta sharp /\
+  (g_adjf1 [:'C,'D:] (idC,compC) (G:('D, 'C, 'G) g_functor)
+                     (eta : ('C, I, 'F o 'G) g_nattransf) sharp /\
     g_functor (idD,compD) (idC,compC) G /\
-    g_nattransf [:'C:] (idC, compC) eta (g_I [:'C:]) (G g_oo F') /\ 
+    g_nattransf [:'C:] (idC, compC) eta (g_I [:'C:])
+                       (G g_oo (F' : ('C, 'D, 'F) g_functor)) /\ 
     (flatt = FLATT (idC, compC) G eta) = 
   g_adjf4 [:'C,'D:] (idC,compC) (idD,compD) sharp flatt /\
     (eta = ETA (idD,compD) flatt) /\ 
     (F' = (\:'a 'b. (\f. sharp (compC eta f)))) /\
     (G = (\:'a 'b. (\g. flatt (compD g (EPS (idC,compC) sharp))))))`` ;
 
+val EPS = ``EPS [:'C, 'D:] (idC,compC) (sharp: ('C,'D, 'F,'G)g_sharp)``
+val ETA = ``ETA [:'D, 'C:] (idC,compC) (flatt: ('D,'C, 'G,'F)g_flatt)``
+val g_adjf1_eq3'' = REWRITE_RULE[GSYM AND_IMP_INTRO]
+                     (MATCH_MP (DECIDE ``(a ==> (b /\ c = d)) ==> (b ==> a ==> c ==> d)``)
+                               g_adjf13_equiv)
+val g_adjf3_eq4'' = REWRITE_RULE[GSYM AND_IMP_INTRO]
+                     (MATCH_MP (DECIDE ``(a ==> (b /\ c = d)) ==> (b ==> c ==> a ==> d)``)
+                               g_adjf34_equiv)
+
+val hyps = strip_conj (fst (dest_imp (concl g_adjf4_3)))
+val theta = foldl (fn (e,tht) => (lhs e |-> subst tht (rhs e)) :: tht
+                                 handle HOL_ERR _ => tht) [] hyps
+val g43' = REWRITE_RULE[GSYM AND_IMP_INTRO] (INST theta g_adjf4_3)
+
+val g_adjf3_eq1' = REWRITE_RULE[GSYM AND_IMP_INTRO]
+                     (MATCH_MP (DECIDE ``(a ==> (b = d)) ==> (b ==> a ==> d)``)
+                               (GSYM g_adjf13_equiv))
+
 (* note that the second and third conditions in g_adjf4 are equivalent,
   in the presence of the first condition - TO BE PROVED *)
 val g_adjf14_equiv = store_thm ("g_adjf14_equiv", tm14e,
-  STRIP_TAC THEN EQ_TAC THEN STRIP_TAC 
-  THENL [
-    EVERY [
-      (USE_LIM_RES_TAC (MAP_EVERY ASSUME_TAC o CONJUNCTS) ( g_adjf1_eq3')),
-      (USE_LIM_RES_TAC (MAP_EVERY ASSUME_TAC o CONJUNCTS) ( g_adjf3_eq4')),
-      (REPEAT CONJ_TAC THEN FIRST_ASSUM ACCEPT_TAC)],
-    EVERY [
-      (USE_LIM_RES_TAC (MAP_EVERY ASSUME_TAC o CONJUNCTS) ( g43)),
-      (POP_ASSUM_LIST (MAP_EVERY (ASSUME_TAC o GSYM))),
-      (FULL_SIMP_TAC simpLib.empty_ss []),
-      (USE_LIM_RES_TAC (MAP_EVERY ASSUME_TAC o CONJUNCTS) 
-        ( (GSYM g_adjf3_eq1))),
-      (REPEAT CONJ_TAC THEN (FIRST_ASSUM ACCEPT_TAC ORELSE REFL_TAC))] ]) ;
-      
+  STRIP_TAC THEN EQ_TAC THEN STRIP_TAC
+  THENL
+    [ ASSUME_TAC (REFL EPS)
+      THEN USE_LIM_RES_TAC STRIP_ASSUME_TAC g_adjf1_eq3''
+      THEN USE_LIM_RES_TAC STRIP_ASSUME_TAC g_adjf3_eq4''
+      THEN REPEAT CONJ_TAC THEN FIRST_ASSUM ACCEPT_TAC,
+
+      USE_LIM_RES_TAC (STRIP_ASSUME_TAC o GSYM) g43'
+      THEN FULL_SIMP_TAC simpLib.empty_ss []
+      THEN USE_LIM_RES_TAC STRIP_ASSUME_TAC (GSYM g_adjf3_eq1')
+      THEN REPEAT CONJ_TAC
+      THEN (FIRST_ASSUM ACCEPT_TAC ORELSE REFL_TAC)
+    ]) ;
+
 (* assumptions of this theorem are the definition of adjoint pair
   currently (Jan 2010) on Wikipedia, under the heading
   Definition via counit-unit adjunction *)
@@ -865,7 +820,8 @@ val tm53 = mk_imp (
   list_mk_conj [adjf5, catC, catD, funF, funG, nteta, nteps], adjf3) ;
 
 (*
-val tm53 = ``g_adjf5 [:'C,'D:] (idC,compC) (idD,compD) F' G eta eps /\
+val tm53 =
+``g_adjf5 [:'C,'D, 'F,'G:] (idC,compC) (idD,compD) F' G eta eps /\
   category (idC,compC) /\ category (idD,compD) /\ 
   g_functor (idC,compC) (idD,compD) F' /\
   g_functor (idD,compD) (idC,compC) G /\
@@ -875,30 +831,35 @@ val tm53 = ``g_adjf5 [:'C,'D:] (idC,compC) (idD,compD) F' G eta eps /\
 *)
 
 val g_adjf5_3 = store_thm ("g_adjf5_3", tm53,
-  EVERY [ (REWRITE_TAC [g_adjf5_thm, g_adjf3_thm]),
-    (REPEAT STRIP_TAC), EQ_TAC,
-    (DISCH_THEN (fn th => REWRITE_TAC [GSYM th])), (farwmmp g_functorD) ]
-  THENL [
-    EVERY [ (farwmmp catDAss),
-      (FIRST_X_ASSUM (CHANGED_TAC o 
-        (fn th => REWRITE_TAC [g_I_thm, I_THM, th]) o REWRITE_RULE [o_THM] o
-	  TY_BETA_RULE o REWRITE_RULE [g_oo_thm] o 
-	  MATCH_MP (GSYM g_nattransfD))),
-      (farwmmp catDRAss)],
-    EVERY [ (farwmmp catDRAss),
-      (FIRST_X_ASSUM (CHANGED_TAC o 
-        (fn th => REWRITE_TAC [g_I_thm, I_THM, th]) o REWRITE_RULE [o_THM] o
-	  TY_BETA_RULE o REWRITE_RULE [g_oo_thm] o MATCH_MP g_nattransfD)),
-      (farwmmp catDAss)] ]
-  THEN (ASM_REWRITE_TAC []) THEN (farwmmp categoryD) ) ;
+  REWRITE_TAC [g_adjf5_thm, g_adjf3_thm]
+  THEN REPEAT STRIP_TAC
+  THEN EQ_TAC
+  THEN DISCH_THEN (REWRITE_THM o GSYM)
+  THEN farwmmp g_functorD
+  THENL
+    [ farwmmp catDAss
+      THEN IMP_RES_THEN (REWRITE_THM o SIMP_RULE combin_ss [g_oo_thm,g_I_def])
+                        (GSYM g_nattransfD)
+      (* PVH: why doesn't the simplifier do g_I_thm? *)
+      THEN farwmmp catDRAss,
+
+      farwmmp catDRAss
+      THEN IMP_RES_THEN (REWRITE_THM o SIMP_RULE combin_ss [g_oo_thm,g_I_def])
+                        g_nattransfD
+      THEN farwmmp catDAss
+    ]
+  THEN ASM_REWRITE_TAC []
+  THEN farwmmp categoryD
+) ;
 
 val tm35 = list_mk_imp ([catC, catD, funF, funG, adjf3], adjf5) ;
 
 val g_adjf3_5= store_thm ("g_adjf3_5", tm35,
-  EVERY [ (REWRITE_TAC [g_adjf5_thm, g_adjf3_thm]),
-    (REPEAT STRIP_TAC) THENL [ (ASM_REWRITE_TAC []), 
-      (FIRST_ASSUM (fn th => CHANGED_TAC (REWRITE_TAC [GSYM th]))) ],
-    (farwmmp g_functorD), (farwmmp categoryD) ]) ;
+  SRW_TAC [] [g_adjf5_thm, g_adjf3_thm]
+  THENL [ ALL_TAC, FIRST_ASSUM (REWRITE_THM o GSYM) ]
+  THEN farwmmp g_functorD
+  THEN farwmmp categoryD
+) ;
 
 (* now to set out our adjoint functor results in the form in the paper *)
 (* first, that the second and third parts of g_adjf4 are equivalent *)
@@ -907,35 +868,38 @@ val g_adjf4_chk = prove (mk_eq (adjf4, list_mk_conj [adjf4a, adjf4b, adjf4c]),
   REWRITE_TAC [g_adjf4_thm]) ;
 
 fun usehs th = 
-  let val (a1,a2) = EQ_IMP_RULE (SPEC_ALL (TY_SPEC_ALL th)) ;
-    fun mk2 ti = DISCH_ALL (TY_GEN_ALL (GEN_ALL (GSYM (inst_eqs (GSYM ti))))) ;
+  let val (a1,a2) = EQ_IMP_RULE (TY_TM_SPEC_ALL th) ;
+    fun mk2 ti = DISCH_ALL (TY_TM_GEN_ALL (GSYM (inst_eqs (GSYM ti)))) ;
     fun tac ui = FIRST_ASSUM (ASSUME_TAC o MATCH_MP ui) ;
   in MAP_EVERY (tac o mk2) [a1, a2] end ;
 
 val g_adjf4_eqv = store_thm ("g_adjf4_eqv",
   list_mk_imp ([cats, adjf4a], mk_eq (adjf4b, adjf4c)),
-  EVERY [REPEAT STRIP_TAC, (FIRST_ASSUM usehs), EQ_TAC, REPEAT STRIP_TAC]
-  THENL [
-    EVERY [ (ONCE_ASM_REWRITE_TAC []),
-      (FIRST_X_ASSUM (fn th => EVERY [CHANGED_TAC (ONCE_REWRITE_TAC [th]),
-	(ASM_REWRITE_TAC []), ASSUME_TAC (GSYM th)])),
-      (farwmmp catDRAss), (ASM_REWRITE_TAC []),
-      (farwmmp catDLU), (ASM_REWRITE_TAC []) ], 
-    EVERY [ 
-      (FIRST_X_ASSUM (fn th => MATCH_MP_TAC 
-        ((fst o EQ_IMP_RULE o SPEC_ALL o TY_SPEC_ALL) th))),
-      (FIRST_X_ASSUM (fn th => EVERY [CHANGED_TAC (ONCE_REWRITE_TAC [th]),
-	(ASM_REWRITE_TAC []), ASSUME_TAC (GSYM th)])),
-      (farwmmp catDAss), (ASM_REWRITE_TAC []),
-      (farwmmp catDRU), (ASM_REWRITE_TAC []) ] ]) ;
+  REPEAT STRIP_TAC
+  THEN FIRST_ASSUM usehs
+  THEN EQ_TAC
+  THEN REPEAT STRIP_TAC
+  THENL
+    [ ONCE_ASM_REWRITE_TAC []
+      THEN POP_ASSUM (fn th => ONCE_REWRITE_TAC [th]
+                               THEN ASM_REWRITE_TAC []
+                               THEN ASSUME_TAC (GSYM th))
+      THEN farwmmp catDRAss
+      THEN ASM_REWRITE_TAC []
+      THEN farwmmp catDLU
+      THEN ASM_REWRITE_TAC [],
 
-(*
-show_types := true ;
-show_types := false ;
-handle e => Raise e ;
-set_goal ([], it) ;
-val (sgs, goal) = top_goal () ;
-*)
+      FIRST_X_ASSUM (MATCH_MP_TAC o fst o EQ_IMP_RULE o TY_TM_SPEC_ALL)
+      THEN POP_ASSUM (fn th => ONCE_REWRITE_TAC [th]
+                               THEN ASM_REWRITE_TAC []
+                               THEN ASSUME_TAC (GSYM th))
+      THEN farwmmp catDAss
+      THEN ASM_REWRITE_TAC []
+      THEN farwmmp catDRU
+      THEN ASM_REWRITE_TAC []
+    ]
+) ;
+
 val taf1 = list_mk_conj [funG, nteta, adjf1, eps, flatt, Feq] ;
 val taf2 = list_mk_conj [funF, nteps, adjf2, eta, sharp, Geq] ;
 val taf3 = list_mk_conj [funF, funG, adjf3, flatt, sharp] ;
@@ -952,107 +916,96 @@ val [g_adjf3e4, g_adjf4e3] = map (REWRITE_RULE [GSYM AND_IMP_INTRO])
 
 val adjf_thm_1_eq_3 = store_thm ("adjf_thm_1_eq_3",
   mk_imp (cats, mk_eq (taf1, taf3)),
-  EVERY [ STRIP_TAC, EQ_TAC, STRIP_TAC ]
-  THENL [
-    EVERY [ REPEAT CONJ_TAC, TRY (FIRST_ASSUM ACCEPT_TAC),
-      (frrc_rewr g_adjf1e3) ],
-    EVERY [ 
-      (FIRST_REP_RES (MAP_EVERY ASSUME_TAC o CONJUNCTS)
-	(REWRITE_RULE [GSYM AND_IMP_INTRO] g_adjf3_nt)),
-      REPEAT CONJ_TAC, TRY (FIRST_ASSUM ACCEPT_TAC),
-      TRY (frrc_rewr g_adjf3e1), (* just one subgoal now *)
-      (FIRST_REP_RES (ASSUME_TAC o CONJUNCT1) g_adjf3e1),
-      (FIRST_REP_RES ASSUME_TAC 
-	(REWRITE_RULE [adjf1_conds_thm, GSYM AND_IMP_INTRO] g_adjf1_Feq)),
-      (CONV_TAC mk_exp_conv''),
-      (FIRST_ASSUM MATCH_ACCEPT_TAC) ] ]) ;
+  STRIP_TAC
+  THEN EQ_TAC
+  THEN STRIP_TAC
+  THENL
+    [ REPEAT CONJ_TAC
+      THEN TRY (FIRST_ASSUM ACCEPT_TAC)
+      THEN frrc_rewr g_adjf1e3,
+
+      IMP_RES_TAC (REWRITE_RULE [GSYM AND_IMP_INTRO] g_adjf3_nt)
+      THEN REPEAT CONJ_TAC
+      THEN TRY (FIRST_ASSUM ACCEPT_TAC)
+      THEN TRY (frrc_rewr g_adjf3e1) (* just one subgoal now *)
+      THEN FIRST_REP_RES (ASSUME_TAC o CONJUNCT1) g_adjf3e1
+      THEN IMP_RES_TAC (REWRITE_RULE [adjf1_conds_thm, GSYM AND_IMP_INTRO] g_adjf1_Feq)
+      THEN POP_ASSUM (REWRITE_THM o GSYM)
+      THEN CONV_TAC (TOP_DEPTH_CONV (ETA_CONV ORELSEC TY_ETA_CONV))
+      THEN REFL_TAC
+    ]
+) ;
 
 val adjf_thm_2_eq_3 = store_thm ("adjf_thm_2_eq_3",
   mk_imp (cats', mk_eq (taf2, taf3')),
-  EVERY [
-    (CONV_TAC (ONCE_DEPTH_CONV (FIRST_CONV (map REWR_CONV dual_convs)))),
-    (REWRITE_TAC [g_oo_dual, g_I_dual]), DISCH_TAC,
-    (FIRST_ASSUM (fn th => REWRITE_TAC [GSYM (MATCH_MP adjf_thm_1_eq_3 th)])),
-    EQ_TAC, STRIP_TAC, ASM_REWRITE_TAC []]
-  THENL [ (REWRITE_TAC [g_dual_functor_def, dual_comp_def]),
-    (FIRST_X_ASSUM (fn th => MP_TAC th THEN CHANGED_TAC 
-      (REWRITE_TAC [g_dual_functor_def, dual_comp_def]))) ]
-  THEN EVERY [ POP_ASSUM_LIST (fn _ => ALL_TAC), TY_BETA_TAC, BETA_TAC]
-  THENL [ REFL_TAC,
-    (CONV_TAC mk_exp_conv'') THEN (SRW_TAC [] []) ]) ;
+  ONCE_REWRITE_TAC dual_convs
+  THEN REWRITE_TAC [g_oo_dual, g_I_dual]
+  THEN DISCH_TAC
+  THEN FIRST_ASSUM (REWRITE_THM o GSYM o MATCH_MP adjf_thm_1_eq_3)
+  THEN EQ_TAC THEN STRIP_TAC THEN ASM_REWRITE_TAC []
+  THENL [ ALL_TAC, POP_ASSUM MP_TAC ]
+  THEN REWRITE_TAC [g_dual_functor_def, dual_comp_def]
+  THEN SIMP_TAC bool_ss []
+  THEN CONV_TAC mk_exp_conv''
+  THEN SIMP_TAC bool_ss []
+) ;
 
 val adjf_thm_3_eq_4 = store_thm ("adjf_thm_3_eq_4",
   mk_imp (cats, mk_eq (taf3, taf4)),
-  EVERY [ STRIP_TAC, EQ_TAC, STRIP_TAC ]
-  THENL [
-    EVERY [ REPEAT CONJ_TAC, TRY (FIRST_ASSUM ACCEPT_TAC),
-      (frrc_rewr g_adjf3e4) ],
-    EVERY [ REPEAT CONJ_TAC, TRY (FIRST_ASSUM ACCEPT_TAC),
-      (frrc_rewr g_adjf4e3) ] ]) ;
+  STRIP_TAC
+  THEN EQ_TAC
+  THEN REPEAT STRIP_TAC
+  THEN TRY (FIRST_ASSUM ACCEPT_TAC)
+  THEN (frrc_rewr g_adjf3e4 ORELSE frrc_rewr g_adjf4e3)
+) ;
 
 val adjf_thm_3_eq_5 = store_thm ("adjf_thm_3_eq_5",
   mk_imp (cats, mk_eq (taf3, taf5)),
-  EVERY [ STRIP_TAC, EQ_TAC, STRIP_TAC ]
-  THENL [
-    EVERY [ 
-      (FIRST_REP_RES (MAP_EVERY ASSUME_TAC o CONJUNCTS)
-	(REWRITE_RULE [GSYM AND_IMP_INTRO] g_adjf3_nt)),
-      (frrc_rewr g_adjf3_5),
-      REPEAT CONJ_TAC, (FIRST_X_ASSUM ACCEPT_TAC) ],
-    EVERY [
-      (FIRST_REP_RES ASSUME_TAC (REWRITE_RULE [GSYM AND_IMP_INTRO] g_adjf5_3)),
-      REPEAT CONJ_TAC, (FIRST_X_ASSUM ACCEPT_TAC) ]]) ;
+  STRIP_TAC
+  THEN EQ_TAC
+  THEN STRIP_TAC
+  THENL
+    [ IMP_RES_TAC (REWRITE_RULE [GSYM AND_IMP_INTRO] g_adjf3_nt)
+      THEN frrc_rewr g_adjf3_5
+      THEN REPEAT CONJ_TAC THEN FIRST_ASSUM ACCEPT_TAC,
 
-(*
-show_types := true ;
-show_types := false ;
-handle e => Raise e ;
-set_goal ([], it) ;
-val (sgs, goal) = top_goal () ;
-*) 
+      IMP_RES_TAC (REWRITE_RULE [GSYM AND_IMP_INTRO] g_adjf5_3)
+      THEN REPEAT CONJ_TAC THEN FIRST_ASSUM ACCEPT_TAC
+    ]
+) ;
 
-(* note - RES_CANON doesn't deal with ty-foralls properly *)
-
-val tgs = TY_GEN_ALL (GEN_ALL FLATT_eps_I) ;
-val rctgs = RES_CANON tgs ; 
-(* takes off the ty-foralls (recent change ?), but doesn't put them back *)
-(* so still need to use seith *)
+(* note - RES_CANON doesn't deal with ty-foralls properly *) (* PVH: now it does *)
 
 val tmjmj = 
-``category (idC, compC) /\ g_functor (idD,compD) (idC,compC) G /\
-  category (idD, compD) /\ g_functor (idC,compC) (idD,compD) F' /\
+``category (idC, compC) /\ g_functor [:'D,'C,'G:] (idD,compD) (idC,compC) G  /\
+  category (idD, compD) /\ g_functor [:'C,'D,'F:] (idC,compC) (idD,compD) F' /\
   g_adjf3 (idC,compC) (idD,compD) F' G (eta : ('C, I, 'F o 'G) g_nattransf)
-    (eps : ('D, 'G o 'F, I) g_nattransf) ==> 
-  (compD eps (F' (G eps)) = compD eps eps)`` ;
+                                       (eps : ('D, 'G o 'F, I) g_nattransf) ==> 
+  (compD (eps [:'a:]) (F' (G eps)) = compD eps eps)`` ;
 
-val g_adjf3_jmj_lem = store_thm ("g_adjf3_jmj_lem", tmjmj, 
-  EVERY [STRIP_TAC,
-    (FIRST_ASSUM (MATCH_MP_TAC o MATCH_MP g_adjf3D1)),
-    (ASSUME_TAC seith), RES_TAC, 
-    (* can't here use (ASSUME_TAC tgs), RES_TAC, *) 
-    REPEAT (FIRST_X_ASSUM (fn th => REWRITE_TAC [MATCH_MP g_functorD th])),
-    REPEAT (FIRST_X_ASSUM (fn th => 
-      ASSUME_TAC (MATCH_MP catDRU th) THEN
-      ASM_REWRITE_TAC [(MATCH_MP catDRAss th)])) ]) ;
-
-val jmjth = DISCH_ALL (TY_GEN_ALL (UNDISCH g_adjf3_jmj_lem)) ;
+val g_adjf3_jmj_lem = store_thm ("g_adjf3_jmj_lem", tmjmj,
+  STRIP_TAC
+  THEN IMP_RES_THEN MATCH_MP_TAC g_adjf3D1
+  THEN IMP_RES_TAC (REWRITE_RULE [GSYM AND_IMP_INTRO] FLATT_eps_I)
+  THEN IMP_RES_THEN REWRITE_THM g_functorD
+  THEN IMP_RES_TAC catDRU
+  THEN IMP_RES_THEN ASM_REWRITE_THM catDRAss
+) ;
 
 (* given adjoint functors, you have a monad *)
 (* NOTE - where do we assume that eta is a natural transformation *)
 
-val tmass = ``category (idC,compC) /\ g_functor (idD,compD) (idC,compC) G /\
-  g_adjf1 (idC,compC) G eta sharp ==> 
-  (sharp (compC (G (sharp h)) k) = compD (sharp h) (sharp k))`` ;
+val tmass = ``category (idC,compC) /\ g_functor [:'D,'C,'G:] (idD,compD) (idC,compC) G /\
+  g_adjf1 (idC,compC) G (eta : ('C, I, 'F o 'G) g_nattransf) sharp ==> 
+  (sharp [:'a,'b:] (compC (G (sharp [:'c,'b:] h)) k) = compD (sharp h) (sharp k))`` ;
 
 val g_adjf1_monad_lem = store_thm ("g_adjf1_monad_lem", tmass,
-  EVERY [ STRIP_TAC,
-    (FIRST_ASSUM (MATCH_MP_TAC o MATCH_MP g_adjf1D1)),
-    (FIRST_X_ASSUM (fn th => REWRITE_TAC [MATCH_MP g_functorD th])),
-    (FIRST_X_ASSUM (fn th => REWRITE_TAC [(MATCH_MP catDRAss th)])),
-    (FIRST_X_ASSUM (fn th => REWRITE_TAC [MATCH_MP g_adjf1DGh th])) ]) ;
-
-val gahe = DISCH_ALL (TY_GEN_ALL (UNDISCH g_adjf1_sharp_eta)) ;
-val gaml = DISCH_ALL (TY_GEN_ALL (GEN_ALL (UNDISCH g_adjf1_monad_lem))) ;
+  STRIP_TAC
+  THEN FIRST_REP_RES MATCH_MP_TAC g_adjf1D1
+  THEN FIRST_REP_RES REWRITE_THM g_functorD
+  THEN FIRST_REP_RES REWRITE_THM catDRAss
+  THEN FIRST_REP_RES REWRITE_THM g_adjf1DGh
+) ;
 
 val tmmon = ``category (idC,compC) /\ 
   g_functor [:'D,'C,'G:] (idD,compD) (idC,compC) G /\
@@ -1060,15 +1013,19 @@ val tmmon = ``category (idC,compC) /\
   Kmonad [:'C, 'F o 'G:] (idC,compC) (eta, \: 'a 'b. G o sharp)`` ;
 
 val g_adjf1_IMP_Kmonad = store_thm ("g_adjf1_IMP_Kmonad", tmmon,
-  EVERY [ (REWRITE_TAC [Kmonad_thm]),
-    (CONV_TAC (REDEPTH_CONV 
-      (REWR_CONV o_THM ORELSEC TY_BETA_CONV ORELSEC BETA_CONV))),
-    STRIP_TAC, (REPEAT CONJ_TAC)]
-  THENL [(FIRST_X_ASSUM (fn th => REWRITE_TAC [MATCH_MP g_adjf1D th])),
-    (IMP_RES_TAC gahe) THEN
-      (FIRST_X_ASSUM (fn th => ASM_REWRITE_TAC [MATCH_MP g_functorD th])), 
-    (IMP_RES_TAC gaml) THEN
-      (FIRST_X_ASSUM (fn th => ASM_REWRITE_TAC [MATCH_MP g_functorD th]))] ) ;
+  SIMP_TAC combin_ss [Kmonad_thm]
+  THEN STRIP_TAC
+  THEN REPEAT CONJ_TAC
+  THENL
+    [ IMP_RES_THEN REWRITE_THM g_adjf1D,
+
+      IMP_RES_TAC g_adjf1_sharp_eta
+      THEN IMP_RES_THEN ASM_REWRITE_THM g_functorD,
+
+      IMP_RES_TAC g_adjf1_monad_lem
+      THEN IMP_RES_THEN ASM_REWRITE_THM g_functorD
+    ]
+) ;
 
 (* given g_adjf1, we get a monad without assuming that eta is a natural
   transformation, but then from the monad, we get that the unit is a natural
@@ -1080,13 +1037,6 @@ val adjf_gives_nt =
   give a monad, in terms of the 7 rule definition of a monad,
   using g_adjf3_jmj_lem *)
 
-(*
-show_types := true ;
-show_types := false ;
-handle e => Raise e ;
-set_goal ([], it) ;
-val (sgs, goal) = top_goal () ;
-*)
 (* given a monad, you have adjoint functors ;
   results in KmonadTheory show that a monad gives:
   the Kleisli category is a category (Komonad_IMP_Kcat)
@@ -1097,11 +1047,10 @@ val (sgs, goal) = top_goal () ;
 val Kmonad_IMP_adjf = store_thm ("Kmonad_IMP_adjf",
   ``Kmonad [:'A, 'M:] (id,comp) (unit,ext) ==> 
     g_adjf1 [:'A, ('A, 'M) Kleisli, I,'M :] (id,comp) ext unit (\: 'a 'b. I)``,
-  EVERY [ (REWRITE_TAC [g_adjf1_def, Kmonad_thm]),
-    (CONV_TAC (REDEPTH_CONV
-      (REWR_CONV UNCURRY_DEF ORELSEC TY_BETA_CONV ORELSEC BETA_CONV))),
-    REPEAT STRIP_TAC, (ASM_REWRITE_TAC [I_THM]),
-    EQ_TAC, (MATCH_ACCEPT_TAC EQ_SYM) ]) ;
+  SIMP_TAC combin_ss [g_adjf1_def, Kmonad_thm, UNCURRY_DEF]
+  THEN STRIP_TAC
+  THEN MATCH_ACCEPT_TAC EQ_SYM_EQ
+) ;
 
 val _ = set_trace "types" 1;
 val _ = set_trace "kinds" 0;
